---
title: "STAT-5361 Homework#8"
author: "Simiao Gao"
output: pdf_document
---

## Exercises 5.3.3

### (1)
$$\mathrm dr(t) = [g(t)+h(t)r(t)] \mathrm dt + \sigma(t) \mathrm dW(t) \\
\text{Hence, } g(t) =\alpha b, \, h(t) =-\alpha,\,\sigma(t)=\sigma \\$$
$$\begin{aligned}

\mathrm d(e^{\alpha t} r(t)) &= e^{\alpha t} \alpha b \,\mathrm dt + e^{\alpha t} \sigma \,\mathrm dW(t) \\
e^{\alpha t} r(t) &= r(0) + \alpha b \int_0^t e^{\alpha s} \,\mathrm ds + \sigma \int_0^t e^{\alpha s} \,\mathrm d W(s) \;\cdots (1)\\
e^{\alpha (t+\Delta)} r(t+\Delta) &= r(0) + \alpha b \int_0^{t+\Delta} e^{\alpha s} \,\mathrm ds + \sigma \int_0^{t+\Delta} e^{\alpha s} \,\mathrm d W(s) \;\cdots (2) 
\end{aligned}$$

$$(2) - (1) \, \implies r(t+\Delta) = e^{-\alpha \Delta} r(t) + b(1-e^{-\alpha}) + \sigma \int_t^{t+\Delta} e^{\alpha s} \,\mathrm d W(s)$$

$$\begin{aligned}
\sigma_r^2(t,t+\Delta) &= \int_t^{t+\Delta} e^{2\alpha (s-t-\Delta)} \,\mathrm ds       \\
&=\frac{\sigma^2}{2\alpha} (1-e^{-2\alpha}) 
\end{aligned}$$

Therefore,
$$r(t+\Delta) = e^{-\alpha \Delta} r(t) + b(1-e^{-\alpha}) + \frac{\sigma}{\sqrt{2\alpha}} \sqrt{1-e^{-2\alpha \Delta}}Z$$



### (2)



```{r message=FALSE, warning=FALSE, tidy=TRUE, tidy.opts=list(width.cutoff=50)}

```

### (3)



```{r message=FALSE, warning=FALSE}

```

